Checkpoint starting to fix waitgroup proof (including admits related to
1.25 upgrade)

new/proof/sync_proof/waitgroup.v
@@ -1,59 +1,46 @@
 From New.proof.sync_proof Require Import base sema.
 From New.experiments Require Import glob.
-<<<<<<< HEAD
-=======
 Local Existing Instances tokG wg_totalG rw_ghost_varG rw_ghost_wlG rw_ghost_rwmutexG  wg_auth_inG.
->>>>>>> master
 
-Section proof.
-Context `{hG:heapGS Σ, !ffi_semantics _ _}.
-Context `{!globalsGS Σ} {go_ctx : GoContext}.
+Section wps.
+Context `{hG: heapGS Σ, !ffi_semantics _ _}.
+Context {sem : go.Semantics} {package_sem : sync.Assumptions}.
+Local Set Default Proof Using "All".
 Context `{!syncG Σ}.
 
-Local Definition enc (waiters counters : Z) : w64 :=
-  word.add (word.slu (W64 counters) (W64 32)) (W64 (uint.Z waiters)).
+Local Definition waitGroupBubbleFlag := 2147483648.
+Example waitGroupBubbleFlag_ok : #waitGroupBubbleFlag = sync.waitGroupBubbleFlag :=
+  eq_refl.
 
-Local Lemma enc_get_counter (waiters counter : Z) :
-  0 <= waiters < 2^31 →
-  W32 (uint.Z (word.sru (enc waiters counter) (W64 32))) = W32 counter.
-Proof. intros. unfold enc. word. Qed.
+Local Definition enc (low high : w32) : w64 :=
+  word.add (word.slu (W64 (uint.Z high)) (W64 32)) (W64 (uint.Z low)).
 
-Local Lemma enc_get_waiters (waiters counter : Z) :
-  0 ≤ waiters < 2^31 →
-  W32 (uint.Z (word.and (enc waiters counter) (W64 2147483647))) = W32 waiters.
-Proof. unfold enc. admit. Admitted.
-
-Local Lemma enc_get_bubble (waiters counter : Z) :
-  0 ≤ waiters < 2^31 →
-  0 ≤ counter < 2^32 →
-  word.and (enc waiters counter) (W64 sync.waitGroupBubbleFlag) = (W64 0).
-Proof.
-  unfold enc. unfold sync.waitGroupBubbleFlag. intros.
-  rewrite Automation.word.word_eq_iff_Z_eq.
-  rewrite word.unsigned_and. rewrite word.unsigned_add.
-  rewrite word.unsigned_slu //.
-  repeat ereplace (uint.Z (W64 ?[x])) with ?x by word.
-Admitted.
-
-Local Lemma enc_add_counter (waiters counter : Z) (delta : w64):
-  word.add (enc waiters counter) (word.slu delta (W64 32)) =
-  enc waiters (counter + sint.Z delta).
+Local Lemma enc_get_high (low high : w32) :
+  W32 (uint.Z (word.sru (enc low high) (W64 32))) = high.
 Proof. unfold enc. word. Qed.
 
-Local Lemma enc_add_waiters (waiters counter : Z) (delta : w64) :
-  word.add (enc waiters counter) delta =
-  enc (waiters + sint.Z delta) counter.
+Local Lemma enc_get_low (low high : w32) :
+  W32 (uint.Z (enc low high)) = low.
 Proof. unfold enc. word. Qed.
 
-Local Lemma enc_inj (waiters counter waiters' counter' : Z) :
-  0 ≤ waiters < 2^31 → 0 ≤ waiters' < 2^31 →
-  0 ≤ counter < 2^32 → 0 ≤ counter' < 2^32 →
-  enc waiters counter = enc waiters' counter' →
-  waiters = waiters' ∧ counter = counter'.
+Local Lemma enc_add_high (low high delta : w32) :
+  word.add (enc low high) (word.slu (W64 (sint.Z delta)) (W64 32)) =
+  enc low (word.add high delta).
+Proof. unfold enc. word. Qed.
+
+Local Lemma enc_add_low (low high delta : w32) :
+  uint.Z (word.add low delta) = uint.Z low + sint.Z delta →
+  word.add (enc low high) (W64 (sint.Z delta)) =
+  enc (word.add low delta) high.
+Proof. unfold enc. word. Qed.
+
+Local Lemma enc_inj (low high low' high' : w32) :
+  enc low high = enc low' high' →
+  low = low' ∧ high = high'.
 Proof. unfold enc. intros. word. Qed.
 
 Local Lemma enc_0 :
-  W64 0 = enc 0 0.
+  W64 0 = enc (W32 0) (W32 0).
 Proof. reflexivity. Qed.
 
 Record WaitGroup_names := {
@@ -65,8 +52,8 @@ Record WaitGroup_names := {
 
 Implicit Type γ : WaitGroup_names.
 
-Definition own_WaitGroup_waiters γ (possible_waiters : Z) : iProp Σ :=
-  own_tok_auth_dfrac γ.(waiter_gn) (DfracOwn (1/2)) (Z.to_nat possible_waiters).
+Definition own_WaitGroup_waiters γ (possible_waiters : w32) : iProp Σ :=
+  own_tok_auth_dfrac γ.(waiter_gn) (DfracOwn (1/2)) (uint.nat possible_waiters).
 #[global] Opaque own_WaitGroup_waiters.
 #[local] Transparent own_WaitGroup_waiters.
 #[global] Instance own_WaitGroup_waiters_timeless γ w : Timeless (own_WaitGroup_waiters γ w) := _.
@@ -78,35 +65,33 @@ Definition own_WaitGroup_wait_token γ : iProp Σ :=
 #[global] Instance own_WaitGroup_wait_token_timeless γ  : Timeless (own_WaitGroup_wait_token γ) := _.
 
 Local Definition is_WaitGroup_inv wg γ N : iProp Σ :=
-  inv (N.@"wg") (∃ (counter waiters possible_waiters : Z) (sema : w32) unfinished_waiters,
+  inv (N.@"wg") (∃ (counter waiters sema possible_waiters : w32) unfinished_waiters,
   "Hsema" ∷ own_sema γ.(sema_gn) sema ∗
   "Hsema_zerotoks" ∷  own_toks γ.(zerostate_gn) (uint.nat sema) ∗
 
-  "Hptsto" ∷ own_Uint64 (struct.field_ref_f sync.WaitGroup "state" wg) (DfracOwn (1/2)) (enc waiters counter) ∗
+  "Hptsto" ∷ own_Uint64 (struct_field_ref sync.WaitGroup.t "state" wg) (DfracOwn (1/2)) (enc waiters counter) ∗
   "Hptsto2" ∷ (
-      if decide (counter = 0 ∧ waiters ≠ 0) then True
-      else own_Uint64 (struct.field_ref_f sync.WaitGroup "state" wg) (DfracOwn (1/2)) (enc waiters counter)
+      if decide (counter = W32 0 ∧ waiters ≠ W32 0) then True
+      else own_Uint64 (struct_field_ref sync.WaitGroup.t "state" wg) (DfracOwn (1/2)) (enc waiters counter)
     ) ∗
   "Hctr" ∷ ghost_var γ.(counter_gn) (1/2)%Qp counter ∗
 
   (* When Add's caller has [own_waiters 0], this resource implies that there are no waiters. *)
-  "Hwait_toks" ∷  own_toks γ.(waiter_gn) (Z.to_nat waiters) ∗
+  "Hwait_toks" ∷  own_toks γ.(waiter_gn) (uint.nat waiters) ∗
   "Hunfinished_wait_toks" ∷ own_toks γ.(waiter_gn) unfinished_waiters ∗
 
   "Hzeroauth" ∷ own_tok_auth γ.(zerostate_gn) unfinished_waiters ∗
 
   (* keeping this to maintain that the number of waiters does not overflow. *)
-  "Hwaiters_bounded" ∷ own_tok_auth_dfrac γ.(waiter_gn) (DfracOwn (1/2)) (Z.to_nat possible_waiters) ∗
+  "Hwaiters_bounded" ∷ own_tok_auth_dfrac γ.(waiter_gn) (DfracOwn (1/2)) (uint.nat possible_waiters) ∗
 
-  "%Hunfinished_zero" ∷ ⌜ unfinished_waiters ≠ O → waiters = 0 ∧ counter = 0 ⌝ ∗
-  "%Hunfinished_bound" ∷ ⌜ Z.of_nat unfinished_waiters < 2^31 ⌝ ∗
-  "%Hpossible_waiters_bounded" ∷ ⌜ 0 ≤ possible_waiters < 2^31 ⌝ ∗
-  "%Hwaiters_bounded" ∷ ⌜ 0 ≤ waiters ⌝ ∗
-  "%Hcounter_bounded" ∷ ⌜ 0 ≤ counter < 2^32 ⌝
+  "%Hunfinished_zero" ∷ ⌜ unfinished_waiters ≠ O → waiters = W32 0 ∧ counter = W32 0 ⌝ ∗
+  "%Hunfinished_bound" ∷ ⌜ Z.of_nat unfinished_waiters < 2^32 ⌝
   )%I.
 
+
 Definition is_WaitGroup wg γ N : iProp Σ :=
-  "#Hsem" ∷ is_sema (struct.field_ref_f sync.WaitGroup "sema" wg) γ.(sema_gn) (N.@"sema") ∗
+  "#Hsem" ∷ is_sema (struct_field_ref sync.WaitGroup.t "sema" wg) γ.(sema_gn) (N.@"sema") ∗
   "#Hinv" ∷ is_WaitGroup_inv wg γ N.
 #[global] Opaque is_WaitGroup.
 #[local] Transparent is_WaitGroup.
@@ -119,31 +104,27 @@ Instance if_sumbool_timeless {PROP : bi} (P Q : PROP) {_:Timeless P} {_:Timeless
 Proof. apply _. Qed.
 
 (* Prepare to Wait() *)
-Lemma alloc_wait_token wg γ N (w : Z) :
-  0 ≤ w < (2^31) - 1 →
+Lemma alloc_wait_token wg γ N (w : w32) :
+  uint.Z (word.add w (W32 1)) = uint.Z w + 1 →
   is_WaitGroup wg γ N -∗
-  own_WaitGroup_waiters γ w ={↑N}=∗ own_WaitGroup_waiters γ (w + 1) ∗ own_WaitGroup_wait_token γ.
+  own_WaitGroup_waiters γ w ={↑N}=∗ own_WaitGroup_waiters γ (word.add w (W32 1)) ∗ own_WaitGroup_wait_token γ.
 Proof.
   intros H. iIntros "[_ #Hinv] H".
   iInv "Hinv" as ">Hi". iNamed "Hi".
   iCombine "Hwaiters_bounded H" gives %[_ ->].
   iCombine "Hwaiters_bounded H" as "H".
   iMod (own_tok_auth_add 1 with "H") as "[H Htok]".
-  iModIntro. rewrite <- (Z2Nat.inj_add _ 1) by word.
-  iDestruct "H" as "[H1 H2]". iSplitR "Htok H2".
-  2:{ by iFrame. } iFrame "∗#%". word.
+  iModIntro. rewrite <- (Z2Nat.inj_add _ 1) by word. rewrite -H.
+  iDestruct "H" as "[H1 H2]". iSplitR "Htok H2"; by iFrame.
 Qed.
 
 Lemma waiters_none_token_false γ :
-  own_WaitGroup_waiters γ 0 -∗ own_WaitGroup_wait_token γ -∗ False.
+  own_WaitGroup_waiters γ (W32 0) -∗ own_WaitGroup_wait_token γ -∗ False.
 Proof.
   iIntros "H1 H2".
   iCombine "H1 H2" gives %H. word.
 Qed.
 
-<<<<<<< HEAD
-Definition own_WaitGroup γ (counter : Z) : iProp Σ :=
-=======
 Lemma dealloc_wait_token wg γ N (w : w32) :
   uint.Z (word.sub w (W32 1)) = uint.Z w - 1 →
   is_WaitGroup wg γ N -∗
@@ -165,63 +146,60 @@ Proof.
 Qed.
 
 Definition own_WaitGroup γ (counter : w32) : iProp Σ :=
->>>>>>> master
   ghost_var γ.(counter_gn) (1/2)%Qp counter.
 #[global] Opaque own_WaitGroup.
 #[local] Transparent own_WaitGroup.
 #[global] Instance own_WaitGroup_timeless γ counter : Timeless (own_WaitGroup γ counter) := _.
 
 Lemma init_WaitGroup N wg_ptr :
-  wg_ptr ↦ (default_val sync.WaitGroup.t) ={⊤}=∗
+  wg_ptr ↦ zero_val sync.WaitGroup.t ={⊤}=∗
   ∃ γ,
-  is_WaitGroup wg_ptr γ N ∗ own_WaitGroup γ 0 ∗ own_WaitGroup_waiters γ 0.
+  is_WaitGroup wg_ptr γ N ∗ own_WaitGroup γ (W32 0) ∗ own_WaitGroup_waiters γ (W32 0).
 Proof.
-  iIntros "H".
-  iDestruct (struct_fields_split with "H") as "H".
-  iNamed "H". simpl.
+  iIntros "H". iStructNamed "H". simpl.
 
-  iMod (ghost_var_alloc 0) as "[%counter_gn [Hctr1 Hctr2]]".
-  iMod (init_sema with "[$Hsema]") as "[%sema_gn [Hs1 Hs2]]".
+  iMod (ghost_var_alloc (W32 0)) as "[%counter_gn [Hctr1 Hctr2]]".
+  iMod (init_sema with "[$sema]") as "[%sema_gn [Hs1 Hs2]]".
   iMod (own_tok_auth_alloc) as "[%waiter_gn [Hwaiters Hw2]]".
   iMod (own_tok_auth_alloc) as "[%zerostate_gn Hzerostate]".
 
   iExists {| sema_gn := sema_gn; counter_gn := counter_gn; zerostate_gn := zerostate_gn; waiter_gn := waiter_gn |}.
   iFrame "∗#".
   unfold is_WaitGroup.
-  iDestruct "Hstate" as "[Hstate Hstate2]".
+  iDestruct "state" as "[state state2]".
   iMod (own_toks_0 waiter_gn) as "?".
   iMod (own_toks_0 waiter_gn) as "?".
   iMod (own_toks_0 zerostate_gn) as "?".
-  iMod (inv_alloc with "[-]") as "$"; last done.
-  iNext. repeat iExists 0. iFrame. simpl. replace (uint.nat (W32 0)) with 0%nat by done. iFrame.
+  iMod (inv_alloc with "[-]") as "$".
+  { iNext. repeat iExists (W32 0). iFrame. done. }
   done.
 Qed.
+
+Local Lemma wg_delta_to_w32 (delta' : w32) (delta : w64) :
+  delta' = (W32 (sint.Z delta)) →
+  word.slu delta (W64 32) = word.slu (W64 (sint.Z delta')) (W64 32).
+Proof. intros. word. Qed.
 
 (* XXX: overflow?
   https://github.com/golang/go/issues/20687
   https://go-review.googlesource.com/c/go/+/140937/2/src/sync/waitgroup.go *)
 
 Lemma wp_WaitGroup__Add (wg : loc) (delta : w64) γ N :
+  let delta' := (W32 (sint.Z delta)) in
   ∀ Φ,
   is_pkg_init sync ∗ is_WaitGroup wg γ N -∗
   (|={⊤,↑N}=>
      ▷ ∃ oldc,
        "Hwg" ∷ own_WaitGroup γ oldc ∗
-<<<<<<< HEAD
-       "%Hbounds" ∷ ⌜ 0 ≤ oldc + sint.Z delta < 2^31 ⌝ ∗
-       "HnoWaiters" ∷ (⌜ oldc ≠ 0 ⌝ ∨ own_WaitGroup_waiters γ 0) ∗
-       "HΦ" ∷ ((⌜ oldc ≠ 0 ⌝ ∨ own_WaitGroup_waiters γ 0) -∗
-               own_WaitGroup γ (oldc + sint.Z delta) ={↑N,⊤}=∗ Φ #())
-=======
        "%Hbounds" ∷ ⌜ 0 ≤ sint.Z oldc + sint.Z delta' < 2^31 ⌝ ∗
        "HΦ" ∷ ((⌜ oldc ≠ W32 0 ⌝ ∗ (own_WaitGroup γ (word.add oldc delta') ={↑N,⊤}=∗ Φ #())) ∨
          (own_WaitGroup_waiters γ (W32 0) ∗
           (own_WaitGroup_waiters γ (W32 0) -∗ own_WaitGroup γ (word.add oldc delta') ={↑N,⊤}=∗
            Φ #())))
->>>>>>> master
   ) -∗
-  WP wg @ (ptrT.id sync.WaitGroup.id) @ "Add" #delta {{ Φ }}.
+  WP wg @! (go.PointerType sync.WaitGroup) @! "Add" #delta {{ Φ }}.
 Proof.
+  intros delta'.
   wp_start as "#His".
   wp_apply wp_with_defer as "%defer defer".
   simpl subst. wp_auto. wp_apply wp_IsInBubble.
@@ -230,17 +208,9 @@ Proof.
   unfold own_WaitGroup.
   iNamed "His".
   iInv "Hinv" as ">Hi" "Hclose".
-<<<<<<< HEAD
-  iNamedSuffix "Hi" "_wg".
-  iApply fupd_mask_intro.
-  { solve_ndisj. }
-  iIntros "Hmask".
-  iCombine "Hctr_wg Hwg" as "Hctr" gives %[_ <-].
-=======
   iApply fupd_mask_intro. { solve_ndisj. } iIntros "Hmask".
   iNext. iNamedSuffix "Hi" "_wg". iNamed "HΦ".
   iCombine "Hctr_wg Hwg" as "Hctr" gives %[_ ->].
->>>>>>> master
   destruct decide as [Hw|HnotInWakingState].
   {
     iExFalso.
@@ -250,8 +220,9 @@ Proof.
     exfalso. apply Hw. word.
   }
   iCombine "Hptsto_wg Hptsto2_wg" as "Hptsto".
-  iExists _. iFrame. rewrite enc_add_counter.
-  iMod (ghost_var_update (counter + sint.Z delta) with "Hctr") as "[Hctr_wg Hwg]".
+  iExists _. iFrame.
+  rewrite (wg_delta_to_w32 delta') // enc_add_high.
+  iMod (ghost_var_update (word.add oldc delta') with "Hctr") as "[Hctr_wg Hwg]".
   iIntros "[Hptsto1_wg Hptsto2_wg]".
   destruct unfinished_waiters.
   2:{
@@ -260,8 +231,7 @@ Proof.
     iCombine "HnoWaiter Hunfinished_wait_toks_wg" gives %Hbad. word.
   }
   subst.
-  iCombine "Hwaiters_bounded_wg Hwait_toks_wg" gives %Hwaiters_bounded.
-  destruct (decide (counter + sint.Z delta = 0 ∧ waiters ≠ 0)) as [Hwake|HnoWake].
+  destruct (decide (word.add oldc delta' = W32 0 ∧ waiters ≠ W32 0)) as [Hwake|HnoWake].
   2:{ (* not done, no need to wake waiters. *)
     iMod "Hmask" as "_".
     iCombineNamed "*_wg" as "Hi".
@@ -269,7 +239,7 @@ Proof.
     {
       iNamed "Hi". iNext. iFrame.
       rewrite decide_False; last intuition.
-      iFrame. iFrame "%". word.
+      iFrame. done.
     }
     iAssert (|={_,_}=> Φ #())%I with "[HΦ Hwg]" as ">HΦ".
     { iDestruct "HΦ" as "[(_ & HΦ)|(? & HΦ)]".
@@ -277,10 +247,7 @@ Proof.
       - iMod ("HΦ" with "[$] [$]"). done. }
     iModIntro.
     wp_auto.
-    rewrite enc_get_bubble; [ | word.. ].
-    wp_auto.
-    rewrite enc_get_counter; [ | word.. ].
-    rewrite enc_get_waiters; [ | word.. ].
+    rewrite enc_get_high enc_get_low.
 
     destruct bool_decide eqn:Hbad.
     {
@@ -301,6 +268,7 @@ Proof.
         wp_auto.
         destruct bool_decide eqn:Heq1.
         + wp_auto. rewrite bool_decide_eq_true in Heq1.
+          replace (W32 (sint.Z delta)) with delta' by reflexivity.
           destruct bool_decide eqn:Heq2.
           * exfalso. rewrite bool_decide_eq_true in Heq2. word.
           * wp_auto. iFrame. done.
@@ -325,18 +293,14 @@ Proof.
   iMod ("Hclose" with "[Hi]") as "_".
   {
     iNamed "Hi". iNext.
-    iFrame. rewrite decide_True; last intuition. word.
+    iFrame. rewrite decide_True; last intuition. done.
   }
     iAssert (|={_,_}=> Φ #())%I with "[HΦ Hwg]" as ">HΦ".
     { iDestruct "HΦ" as "[(_ & HΦ)|(? & HΦ)]".
       - iMod ("HΦ" with "[$]"). done.
       - iMod ("HΦ" with "[$] [$]"). done. }
   iModIntro.
-  wp_auto.
-  rewrite enc_get_bubble; [ | word.. ].
-  wp_auto.
-  rewrite enc_get_counter; [ | word.. ].
-  rewrite enc_get_waiters; [ | word.. ].
+  wp_auto. rewrite enc_get_high enc_get_low.
 
   destruct bool_decide eqn:Hbad.
   { exfalso. rewrite bool_decide_eq_true in Hbad. word. }
@@ -353,6 +317,7 @@ Proof.
       wp_auto.
       destruct bool_decide eqn:Heq1.
       + wp_auto.
+        replace (W32 (sint.Z delta)) with delta' by reflexivity.
         rewrite bool_decide_eq_true in Heq1.
         destruct bool_decide eqn:Heq2.
         * exfalso. rewrite bool_decide_eq_true in Heq2. word.
@@ -388,8 +353,7 @@ Proof.
   iNamedSuffix "Hi" "_wg".
   iClear "Hptsto2_wg".
   iCombine "Hptsto Hptsto_wg"  gives %[_ Heq].
-  iCombine "Hwaiters_bounded_wg Hwait_toks_wg" gives %Hwaiters0_bounded.
-  apply enc_inj in Heq as [<- <-]; [|word..].
+  apply enc_inj in Heq as [<- <-].
   iCombine "Hptsto Hptsto_wg" as "Hptsto".
   iExists _. iFrame.
   iIntros "Hptsto".
@@ -401,7 +365,7 @@ Proof.
   iCombine "Hzeroauth_wg Hsema_zerotoks_wg" gives %Hs.
   replace (sema) with (W32 0) by word.
   clear Huf Hs unfinished_waiters sema.
-  iMod (own_tok_auth_add (Z.to_nat waiters) with "[$Hzeroauth_wg]") as "[Hzeroauth_wg Hzerotoks_wg]".
+  iMod (own_tok_auth_add (uint.nat waiters) with "[$Hzeroauth_wg]") as "[Hzeroauth_wg Hzerotoks_wg]".
   iEval (rewrite enc_0) in "Hptsto".
   iDestruct "Hptsto" as "[Hptsto1_wg Hptsto2_wg]".
   destruct Hwake as [Hwake1 Hwake2].
@@ -416,12 +380,10 @@ Proof.
   (* call semrelease. *)
 
   iAssert (
-      ∃ (wrem : Z),
-        "w" ∷ w_ptr ↦ (W32 wrem) ∗
-        "Hzerotoks" ∷ own_toks γ.(zerostate_gn) (Z.to_nat wrem) ∗
-        "%Hwrem_bounds" ∷ ⌜ 0 ≤ wrem < 2^32 ⌝
-    )%I with "[w Hzerotoks]" as "HloopInv".
-  { iFrame. word. }
+      ∃ (wrem : w32),
+        "w" ∷ w_ptr ↦ wrem ∗
+        "Hzerotoks" ∷ own_toks γ.(zerostate_gn) (uint.nat wrem)
+    )%I with "[$]" as "HloopInv".
 
   wp_for.
   iNamed "HloopInv".
@@ -446,7 +408,7 @@ Proof.
   iExists _; iFrame "Hsema_wg".
   iIntros "Hsema_wg".
   iMod "Hmask" as "_".
-  replace (Z.to_nat wrem)%nat with (1+(Z.to_nat (wrem - 1)))%nat by word.
+  replace (uint.nat wrem)%nat with (1+(uint.nat (word.sub wrem (W32 1))))%nat by word.
   iDestruct (own_toks_add with "Hzerotoks") as "[Hzerotok Hzerotoks]".
   iCombine "Hsema_zerotoks_wg Hzerotok" as "Hsema_zerotok_wg".
   iCombine "Hzeroauth_wg Hsema_zerotok_wg" gives %Hbound.
@@ -458,41 +420,22 @@ Proof.
     iFrame. done.
   }
   iModIntro. wp_auto. wp_for_post. iFrame.
-  iSplitL; last word.
-  iApply to_named. iExactEq "w". f_equal. word.
 Qed.
 
 Lemma wp_WaitGroup__Done (wg : loc) γ N :
   ∀ Φ,
   is_pkg_init sync ∗ is_WaitGroup wg γ N -∗
   (|={⊤,↑N}=>
-<<<<<<< HEAD
-     ∃ counter,
-       "Hwg" ∷ own_WaitGroup γ counter ∗
-       "%Hbounds" ∷ ⌜ 0 ≤ counter - 1 < 2^31 ⌝ ∗
-       "HnoWaiters" ∷ (⌜ counter ≠ 0 ⌝ ∨ own_WaitGroup_waiters γ 0) ∗
-       "HΦ" ∷ ((⌜ counter ≠ 0 ⌝ ∨ own_WaitGroup_waiters γ 0) -∗
-               own_WaitGroup γ (counter - 1) ={↑N,⊤}=∗ Φ #())
-=======
      ▷ ∃ oldc,
        "Hwg" ∷ own_WaitGroup γ oldc ∗
        "%Hbounds" ∷ ⌜ 0 ≤ sint.Z oldc - 1 < 2^31 ⌝ ∗
        "HΦ" ∷ (own_WaitGroup γ (word.sub oldc (W32 1)) ={↑N,⊤}=∗ Φ #())
->>>>>>> master
   ) -∗
   WP wg @ (ptrT.id sync.WaitGroup.id) @ "Done" #() {{ Φ }}.
 Proof.
   wp_start as "#His".
   wp_auto.
   wp_apply (wp_WaitGroup__Add with "[$]").
-<<<<<<< HEAD
-  iMod "HΦ". iNamed "HΦ".
-  change (sint.Z (W64 (-1))) with (-1).
-  iModIntro. iFrame "Hwg HnoWaiters". iSplitR.
-  { word. }
-  iIntros "Hw Hctr".
-  iMod ("HΦ" with "[$] [$]") as "HΦ".
-=======
   iMod "HΦ". iModIntro. iNext. iNamed "HΦ".
   replace (W32 (uint.Z (W64 (-1)))) with (W32 (-1)) by done.
   replace (sint.Z (W32 (-1))) with (-1) by done.
@@ -500,7 +443,6 @@ Proof.
   iLeft. iSplitR; first word. iIntros "Hctr".
   iMod ("HΦ" with "[Hctr]") as "HΦ".
   { iExactEq "Hctr". repeat f_equal. word. }
->>>>>>> master
   iModIntro. wp_auto. iApply "HΦ".
 Qed.
 
@@ -508,22 +450,21 @@ Lemma wp_WaitGroup__Wait (wg : loc) γ N :
   ∀ Φ,
   is_pkg_init sync ∗ is_WaitGroup wg γ N ∗ own_WaitGroup_wait_token γ -∗
   (|={⊤∖↑N, ∅}=>
-<<<<<<< HEAD
-     ∃ counter,
-       own_WaitGroup γ counter ∗ (⌜ counter = 0 ⌝ → own_WaitGroup γ counter ={∅,⊤∖↑N}=∗
-=======
      ▷ ∃ oldc,
        own_WaitGroup γ oldc ∗ (⌜ sint.Z oldc = 0 ⌝ → own_WaitGroup γ oldc ={∅,⊤∖↑N}=∗
->>>>>>> master
                                own_WaitGroup_wait_token γ -∗ Φ #())
   ) -∗
   WP wg @ (ptrT.id sync.WaitGroup.id) @ "Wait" #() {{ Φ }}.
 Proof.
   wp_start as "(#Hwg & HR_in)". iNamed "Hwg".
-  wp_auto. wp_for. wp_apply (wp_Uint64__Load).
+  wp_auto.
+  wp_for_core. (* TODO: need to set later credits *)
+  wp_auto.
+  rewrite decide_True //. wp_auto.
+  wp_apply (wp_Uint64__Load).
   iInv "Hinv" as ">Hi" "Hclose".
   iNamedSuffix "Hi" "_wg".
-  destruct (decide (counter = 0)).
+  destruct (decide (counter = W32 0)).
   { (* counter is zero, so can return. *)
     subst.
 
@@ -536,20 +477,14 @@ Proof.
     iIntros "Hptsto_wg".
     iMod ("HΦ" with "[//] [$Hwg]") as "HΦ".
     iMod "Hmask" as "_".
-    iCombine "Hwaiters_bounded_wg Hwait_toks_wg" gives %Hwaiters_bounded.
     iCombineNamed "*_wg" as "Hi".
     iMod ("Hclose" with "[Hi]").
     { iNamed "Hi". by iFrame. }
     iModIntro.
+    wp_auto. rewrite enc_get_high enc_get_low bool_decide_true //=.
     wp_auto.
-    rewrite enc_get_counter; [|word..].
-    rewrite enc_get_waiters; [|word..].
-    wp_auto.
-    wp_bind (if: if: if: _ then _ else _ then _ else _ then _ else _)%E.
-    iApply (wp_wand _ _ _ (λ v, ⌜ v = execute_val ⌝ ∗ _)%I with "[-]").
-    { wp_if_destruct. 2:{ iSplitR; first done. iNamedAccu. } wp_auto.
-      rewrite enc_get_bubble; [ | word.. ]. wp_auto. iFrame. done. }
-    iIntros "% [-> H]". iNamed "H". wp_auto. wp_for_post. by iApply "HΦ".
+    wp_for_post.
+    by iApply "HΦ".
   }
   (* actually go to sleep *)
   iApply fupd_mask_intro.
@@ -567,11 +502,10 @@ Proof.
   { iNamed "Hi". by iFrame. }
   iModIntro.
   wp_auto.
-  rewrite enc_get_counter; [|word..].
-  rewrite enc_get_waiters; [|word..].
-  rewrite bool_decide_false; [|word..].
+  rewrite enc_get_high enc_get_low bool_decide_false //.
   wp_auto.
-  rewrite enc_add_waiters; [|word..].
+  replace (1%Z) with (sint.Z (W32 1)) by reflexivity.
+  rewrite -> enc_add_low by word.
   wp_apply (wp_Uint64__CompareAndSwap).
   iInv "Hinv" as ">Hi" "Hclose".
   iNamedSuffix "Hi" "_wg".
@@ -582,8 +516,7 @@ Proof.
   iExists (enc waiters0 counter0).
   destruct (decide (_ = _)) as [Heq|Hneq].
   {
-    iCombine "Hwaiters_bounded_wg Hwait_toks_wg" gives %Hwaiters0_bounded.
-    apply enc_inj in Heq as [-> ->]; [|word..].
+    apply enc_inj in Heq as [-> ->].
     rewrite decide_False.
     2:{ naive_solver. }
     iCombine "Hptsto_wg Hptsto2_wg" as "$".
@@ -595,17 +528,18 @@ Proof.
     iMod ("Hclose" with "[Hi]") as "_".
     {
       iNext. iNamed "Hi". repeat iExists _. iFrame "Hptsto_wg ∗".
-      replace (Z.to_nat (waiters + sint.Z (W64 1))) with (1 + Z.to_nat waiters)%nat by word.
-      simpl. iFrame. iSplitL.
+      replace (uint.nat (word.add waiters (W32 1))) with (1 + uint.nat waiters)%nat by word.
+      simpl. iFrame.
+      iSplitL.
       { by destruct decide. }
-      iPureIntro. word.
+      iPureIntro. split; last done.
+      intros Hun. exfalso. naive_solver.
     }
     iModIntro.
     wp_auto.
     clear sema n unfinished_waiters Hunfinished_zero_wg Hunfinished_bound_wg
                unfinished_waiters0 Hunfinished_zero_wg0 Hunfinished_bound_wg0.
 
-    rewrite enc_get_bubble; [ | word.. ]. wp_auto.
     wp_apply (wp_runtime_SemacquireWaitGroup with "[$]").
     iInv "Hinv" as ">Hi" "Hclose".
     iNamedSuffix "Hi" "_wg".
@@ -630,7 +564,7 @@ Proof.
     wp_auto.
     wp_apply (wp_Uint64__Load).
     iInv "Hinv" as ">Hi" "Hclose".
-    iClear "v w state". clear dependent v_ptr counter w_ptr waiters state_ptr.
+    iClear "v w state". clear v_ptr counter w_ptr waiters state_ptr HwaitersLe.
     clear unfinished_waiters sema n Hsema Hsem Hunfinished_zero_wg Hunfinished_bound_wg.
     iNamedSuffix "Hi" "_wg".
     iMod (fupd_mask_subseteq _) as "Hmask"; last iMod "HΦ" as (?) "[Hwg HΦ]".
